cava/Cava/Lib/RetimingProperties.v
@@ -47,9 +47,17 @@ All should be based on phase_retimed!
 
  *)
 
+Lemma cpath_delays {t} : cpath (@delays _ _ t) = 1.
+Proof.
+  induction t; cbn [delays cpath Delay Par]; [ reflexivity .. | ].
+Qed.
+
 Lemma move_delays {i o} (c : Circuit i o) :
   is_loop_free c = true -> wequiv (delays >==> c) (c >==> delays).
-Admitted.
+Proof.
+  intros. cbv [wequiv]. ssplit; [ cbn [cpath]; try lia | ].
+  { Set Printing All.
+Qed.
 
 Lemma split_ndelays {t1 t2} n :
   wequiv (ndelays (t:=t1 * t2) n) (Par (ndelays n) (ndelays n)).
@@ -69,6 +77,130 @@ Lemma delayn_input {i o} n m (c1 c2 : Circuit i o) :
   phase_retimed n 0 c1 (ndelays m >==> c2) ->
   phase_retimed n m c1 c2.
 Admitted.
+
+Lemma Par_Id_l_w {i o t} (f : Circuit i o) : wequiv (Par f (Id (t:=t))) (First f).
+Proof. cbv [Par]. autorewrite with circuitsimplw. reflexivity. Qed.
+Hint Rewrite @Par_Id_l_w using solve [eauto] : circuitsimplw.
+
+Lemma Par_Id_r_w {i o t} (f : Circuit i o) : wequiv (Par (Id (t:=t)) f) (Second f).
+Proof. cbv [Par]. autorewrite with circuitsimplw. reflexivity. Qed.
+Hint Rewrite @Par_Id_r_w using solve [eauto] : circuitsimplw.
+
+Lemma Second_Comb_w {i o t} f :
+  wequiv (Second (Comb f)) (Comb (i:=t*i) (o:=t*o) (fun x => (fst x, f (snd x)))).
+Proof.
+  cbv [wequiv]. cbn. ssplit; intros; [ reflexivity | ].
+  exists (fun i _ _ => i = 0); ssplit; intros; cbn [step fst snd]; try tauto; lia.
+Qed.
+Hint Rewrite @Second_Comb_w using solve [eauto] : pull_comb.
+
+Lemma First_Comb_w {i o t} f :
+  wequiv (First (Comb f)) (Comb (i:=i*t) (o:=o*t) (fun x => (f (fst x), snd x))).
+Proof.
+  cbv [wequiv]. cbn. ssplit; intros; [ reflexivity | ].
+  exists (fun i _ _ => i = 0); ssplit; intros; cbn [step fst snd]; try tauto; lia.
+Qed.
+Hint Rewrite @First_Comb_w using solve [eauto] : pull_comb.
+
+Lemma Compose_Comb_w {i t o} f g :
+  wequiv (@Compose _ _ i t o (Comb f) (Comb g)) (Comb (f >=> g)).
+Proof.
+  cbv [wequiv]. cbn. ssplit; intros; [ reflexivity | ].
+  exists (fun i _ _ => i = 0); ssplit; intros; cbn [step fst snd]; try tauto; lia.
+Qed.
+Hint Rewrite @Compose_Comb_w using solve [eauto] : pull_comb.
+
+Lemma Compose_Comb_r_w {i t1 t2 o} c f g :
+  wequiv (@Compose _ _ i t2 o (@Compose _ _ i t1 t2 c (Comb f)) (Comb g))
+         (c >==> Comb (f >=> g)).
+Proof.
+  rewrite <-Compose_Comb_w. autorewrite with circuitsimplw. reflexivity.
+Qed.
+Hint Rewrite @Compose_Comb_r_w using solve [eauto] : pull_comb.
+
+Lemma First_Second_comm {i1 i2 o1 o2} (c1 : Circuit i1 o1) (c2 : Circuit i2 o2) :
+  wequiv (First c1 >==> Second c2) (Second c2 >==> First c1).
+Admitted.
+
+Lemma delays_Comb_comm {i o} (f : value i -> cava (value o)) :
+  wequiv (delays >==> Comb f) (Comb f >==> delays).
+Proof.
+  Print wequiv.
+  Search cequivn.
+  induction i.
+  induction n; cbn [ndelays]; autorewrite with circuitsimplw; [ reflexivity | ].
+  rewrite <-(Compose_assoc_w _ _ _ _ (ndelays _) delays).
+Qed.
+
+Lemma ndelays_Comb_comm {i o} (f : value i -> cava (value o)) n :
+  wequiv (ndelays n >==> Comb f) (Comb f >==> ndelays n).
+Proof.
+  induction n; cbn [ndelays]; autorewrite with circuitsimplw; [ reflexivity | ].
+  rewrite <-(Compose_assoc_w _ _ _ _ (ndelays _) delays).
+Qed.
+
+Lemma Comb_ext {i o} (f g : value i -> cava (value o)) :
+  (forall x, f x = g x) -> wequiv (Comb f) (Comb g).
+Proof.
+  intro Hext. cbv [wequiv]. cbn. ssplit; intros; [ reflexivity | ].
+  exists (fun i _ _ => i = 0); ssplit; intros; cbn [step fst snd]; auto; lia.
+Qed.
+
+Lemma loopless_LoopInit {i o s} (body : Circuit (i * s) (o * s)) r :
+  wequiv (loopless (LoopInit r body))
+         (Comb (i:=(_*(_*(_*_)))) (o:=_*_*_)
+               (fun '(x, (_, (body_st, loop_st))) => (x, loop_st, body_st))
+               >==> loopless body
+               >==> (Comb (i:=_*_*_) (o:=(_*(tzero*(_*_))))
+                          (fun '(x, loop_st, body_st) => (x, (tt, (body_st, loop_st)))))).
+Proof.
+  cbv [wequiv]. ssplit; intros; [ cbn; lia | ].
+  cbn [cpath loopless LoopInit]. autorewrite with natsimpl. simpl_ident.
+  cbv [cequivn]. cbn [value loops_state LoopInit circuit_state].
+  destruct (cequivn_reflexive (loopless body) ltac:(apply is_loop_free_loopless))
+    as [Rb ?]. logical_simplify.
+  exists (fun i s1 s2 => Rb i (snd (fst (snd (fst s1)))) (snd (fst s2))).
+  ssplit.
+  { intros; destruct_products. cbn. auto. }
+  { intros; destruct_products. cbn.
+    repeat lazymatch goal with x : unit |- _ => destruct x end.
+    repeat destruct_pair_let. cbn [fst snd].
+    lazymatch goal with H : cpath _ = 0 -> _ |- _ => erewrite H by auto end.
+    reflexivity. }
+  { intros; destruct_products; cbn.
+    repeat lazymatch goal with x : unit |- _ => destruct x end.
+    repeat destruct_pair_let. cbn [fst snd] in *.
+    lazymatch goal with H : forall _ _ _ _, Rb 1 _ _ -> _ |- _ =>
+                        erewrite H by eauto end.
+    reflexivity. }
+  { intros; destruct_products; cbn.
+    repeat lazymatch goal with x : unit |- _ => destruct x end.
+    repeat destruct_pair_let. cbn [fst snd] in *. eauto. }
+Qed.
+
+Lemma retime_loop {i o s} (f g : Circuit (i * s) (o * s)) n r :
+  phase_retimed n n f g ->
+  phase_retimed n n (LoopInit r f) (LoopInit r g).
+Proof.
+  cbv [phase_retimed]. intros [proj_gf [proj_fg [Hproj Hequiv]]].
+  cbn [loops_state value LoopInit].
+  exists (fun x => (fst x, (proj_gf (fst (snd x)), snd (snd x)))).
+  exists (fun x => (fst x, (proj_fg (fst (snd x)), snd (snd x)))).
+  rewrite !loopless_LoopInit. rewrite Hequiv.
+  split; [ intros; destruct_products; cbn [fst snd]; rewrite Hproj;
+           reflexivity | ].
+  autorewrite with circuitsimplw pull_comb.
+  cbv [mcompose]; simpl_ident.
+  (* RHS has delays and Comb flipped around *)
+  repeat eapply Proper_Compose.
+  (* need Proper_comb with funext *)
+  (* each subcircuit should now be equiivalent *)
+  eapply Proper_Comb.
+  Print phase_retimed.
+  (* objective: get to Second (Par (ndelays n) (ndelays n)) >==> loopless g) and rewrite *)
+  
+  Search LoopInitCE.
+Qed.
 
 Instance phase_retimed_0_refl {i o} : Reflexive (@phase_retimed i o 0 0) | 10.
 Proof.
@@ -148,6 +280,7 @@ Proof.
   destruct_lists_by_length. cbn [ndelays] in *.
   cbv [Par] in *; autorewrite with circuitsimplw in *.
   rewrite ndelays_First.
+  Print phase_retimed.
 
   (* TODO: not quite working right now, how to properly incorporate retimed
      subcomponents? *)
